Faithfulness/Rejected/BadSortUniverse.lean
@@ -1,0 +1,8 @@
+namespace LeanLeanFaithfulness.Rejected
+
+universe u
+
+inductive BadPolyBox (α : Sort u) : Sort u
+| mk : α → BadPolyBox α
+
+end LeanLeanFaithfulness.Rejected
